progress on donate

theories/RAs.v
@@ -1434,13 +1434,88 @@ Qed.
 
   (* predicates for descriptors *)
 
+  Definition serialized_memory_descirptor l (r:VMID) ps := [l; (of_imm (encode_vmid r))]++ (map (λ pid, (of_pid pid)) ps).
+
   Definition serialized_transaction_descriptor (v r:VMID) (wf wt l : Word) (ps: list PID) (h : handle ): list Word :=
-    [(of_imm (encode_vmid v)); wf; h;wt; W1%f; l; (of_imm (encode_vmid r))]++ (map (λ pid, (of_pid pid)) ps).
+    [(of_imm (encode_vmid v)); wf; h;wt; W1%f] ++ (serialized_memory_descirptor l r ps).
+
+  Lemma trans_desc_length{i j wf wt l ps} des :
+    des = serialized_transaction_descriptor i j wf wt l ps W0 ->
+    (finz.to_z l) = (Z.of_nat (length ps)) ->
+    ((Z.of_nat (length des)) = 5 + 2 + (finz.to_z l))%Z.
+  Proof.
+    intros.
+    rewrite H /serialized_transaction_descriptor /serialized_memory_descirptor H0.
+    simpl.
+    rewrite fmap_length.
+    lia.
+  Qed.
+
 
   Definition mem_region (instr: list Word) (b:Addr):=
     ([∗ list] a;w ∈ (finz.seq b (length instr));instr, (a ->a w))%I.
 
   Definition transaction1 (v r:VMID) (wf wt l : Word) (rs: list VMID) (ps: list PID)  (ty: transaction_type): transaction :=
     (v,wf,wt,(list_to_set rs),{[r := (list_to_set ps)]},ty).
+
+  Lemma transaction_descriptor_valid{i j wf wt l psd σ} des p :
+    (finz.to_z l) = (Z.of_nat (length psd)) ->
+    des = serialized_transaction_descriptor i j wf wt l psd W0 ->
+    seq_in_page (of_pid p) (length des) p ->
+   (∀ (k : nat) (y1 y2 : Addr),
+             finz.seq (of_pid p) (length des) !! k = Some y1 → des !! k = Some y2 → get_mem σ !! y1 = Some y2) ->
+   parse_transaction_descriptor σ p = Some (i ,  None, wt , wf, W1, ∅).
+  Proof.
+    intros.
+    rewrite /parse_transaction_descriptor /get_memory_with_offset.
+    destruct H1 as [_ [? _]].
+    pose proof (trans_desc_length des H0 H) as Hlen.
+    assert (HpSome: ((of_pid p) + 0)%f = Some ((of_pid p) ^+ 0)%f).
+    solve_finz.
+    rewrite HpSome //=;clear HpSome.
+    rewrite (H2 0 ((of_pid p) ^+ 0)%f (encode_vmid i)).
+    2: { apply finz_seq_lookup. lia. solve_finz. }
+    2: { rewrite H0 /serialized_transaction_descriptor. by list_simplifier. }
+    assert (HpSome: ((of_pid p) + 1)%f = Some ((of_pid p) ^+ 1)%f).
+    solve_finz.
+    rewrite HpSome //=;clear HpSome.
+    rewrite (H2 1 ((of_pid p) ^+ 1)%f wf).
+    2: { apply finz_seq_lookup. lia. solve_finz. }
+    2: { rewrite H0 /serialized_transaction_descriptor. by list_simplifier. }
+    assert (HpSome: ((of_pid p) + 2)%f = Some ((of_pid p) ^+ 2)%f).
+    solve_finz.
+    rewrite HpSome //=;clear HpSome.
+    rewrite (H2 2 ((of_pid p) ^+ 2)%f W0).
+    2: { apply finz_seq_lookup. lia. solve_finz. }
+    2: { rewrite H0 /serialized_transaction_descriptor. by list_simplifier. }
+    assert (HpSome: ((of_pid p) + 3)%f = Some ((of_pid p) ^+ 3)%f).
+    solve_finz.
+    rewrite HpSome //=;clear HpSome.
+    rewrite (H2 3 ((of_pid p) ^+ 3)%f wt).
+    2: { apply finz_seq_lookup. lia. solve_finz. }
+    2: { rewrite H0 /serialized_transaction_descriptor. by list_simplifier. }
+    assert (HpSome: ((of_pid p) + 4)%f = Some ((of_pid p) ^+ 4)%f).
+    solve_finz.
+    rewrite HpSome //=;clear HpSome.
+    rewrite (H2 4 ((of_pid p) ^+ 4)%f W1).
+    2: { apply finz_seq_lookup. lia. solve_finz. }
+    2: { rewrite H0 /serialized_transaction_descriptor. by list_simplifier. }
+    rewrite /parse_memory_region_descriptors //= /parse_memory_region_descriptor /get_memory_with_offset.
+    assert (HpSome: ((of_pid p) + (5 + (0%nat + 0)))%f = Some ((of_pid p) ^+ 5)%f).
+    solve_finz.
+    rewrite HpSome //=;clear HpSome.
+    rewrite (H2 5 ((of_pid p) ^+ 5)%f l).
+    2: { apply finz_seq_lookup. lia. solve_finz. }
+    2: { rewrite H0 /serialized_transaction_descriptor. by list_simplifier. }
+    assert (HpSome: ((of_pid p) + (5 + (0%nat + 0)+1))%f = Some ((of_pid p) ^+ 6)%f).
+    solve_finz.
+    rewrite HpSome //=;clear HpSome.
+    rewrite (H2 6 ((of_pid p) ^+ 6)%f (encode_vmid j)).
+    2: { apply finz_seq_lookup. lia. solve_finz. }
+    2: { rewrite H0 /serialized_transaction_descriptor. by list_simplifier. }
+    rewrite !decode_encode_vmid.
+    (* TODO: need a helper lemma. *)
+    Admitted.
+  
 
 End hyp_lang_rules.
